wip: rsapss

code/rsapss/Hacl.Impl.RSAPSS.Keys.fst
@@ -8,7 +8,6 @@ open Lib.IntTypes
 open Lib.Buffer
 
 open Hacl.Bignum.Definitions
-open Hacl.Bignum
 
 module ST = FStar.HyperStack.ST
 module B = LowStar.Buffer
@@ -22,63 +21,117 @@ module BB = Hacl.Spec.Bignum.Base
 
 #reset-options "--z3rlimit 50 --fuel 0 --ifuel 0"
 
+inline_for_extraction noextract
+val rsapss_check_pkey_len:
+    #t:limb_t
+  -> modBits:size_t{0 < v modBits}
+  -> eBits:size_t{0 < v eBits} ->
+  res:bool{
+    let bits = size (bits t) in
+    let nLen = blocks modBits bits in
+    let eLen = blocks eBits bits in
+    res <==> LS.pkey_len_pre t (v modBits) (v eBits)}
 
-val bn_check_num_bits:
-    bits:size_t{0 < v bits /\ 64 * v (blocks bits 64ul) <= max_size_t}
-  -> b:lbignum (blocks bits 64ul) ->
-  Stack uint64
+let rsapss_check_pkey_len #t modBits eBits =
+  [@inline_let] let bits = size (bits t) in
+  let nLen = blocks modBits bits in
+  let eLen = blocks eBits bits in
+
+  1ul <. modBits && 0ul <. eBits &&
+  nLen <=. 0xfffffffful /. (2ul *! bits) && eLen <=. 0xfffffffful /. bits &&
+  nLen +! nLen <=. 0xfffffffful -. eLen
+
+
+inline_for_extraction noextract
+val rsapss_check_skey_len:
+    #t:limb_t
+  -> modBits:size_t{0 < v modBits}
+  -> eBits:size_t{0 < v eBits}
+  -> dBits:size_t{0 < v dBits} ->
+  res:bool{
+    let bits = size (bits t) in
+    let nLen = blocks modBits bits in
+    let eLen = blocks eBits bits in
+    let dLen = blocks dBits bits in
+    res <==> LS.skey_len_pre t (v modBits) (v eBits) (v dBits)}
+
+let rsapss_check_skey_len #t modBits eBits dBits =
+  [@inline_let] let bits = size (bits t) in
+  let nLen = blocks modBits bits in
+  let eLen = blocks eBits bits in
+  let dLen = blocks dBits bits in
+
+  rsapss_check_pkey_len #t modBits eBits &&
+  0ul <. dBits && dLen <=. 0xfffffffful /. bits &&
+  nLen +! nLen <=. 0xfffffffful -. eLen -. dLen
+
+
+inline_for_extraction noextract
+let bn_check_num_bits_st (t:limb_t) =
+    bs:size_t{0 < v bs /\ bits t * v (blocks bs (size (bits t))) <= max_size_t}
+  -> b:lbignum t (blocks bs (size (bits t))) ->
+  Stack (limb t)
   (requires fun h -> live h b)
   (ensures  fun h0 r h1 -> modifies0 h0 h1 /\
-    r == LS.bn_check_num_bits (v bits) (as_seq h0 b))
-
-[@CInline]
-let bn_check_num_bits bits b =
-  let bLen = blocks bits 64ul in
-  if bits =. 64ul *! bLen then ones U64 SEC else bn_lt_pow2_mask bLen b bits
+    r == LS.bn_check_num_bits (v bs) (as_seq h0 b))
 
 
-val rsapss_check_modulus:
-    modBits:size_t{0 < v modBits /\ 64 * v (blocks modBits 64ul) <= max_size_t}
-  -> n:lbignum (blocks modBits 64ul) ->
-  Stack uint64
+inline_for_extraction noextract
+val bn_check_num_bits: #t:limb_t -> bn_check_num_bits_st t
+let bn_check_num_bits #t bs b =
+  [@inline_let] let bits = size (bits t) in
+  let bLen = blocks bs bits in
+  if bs =. bits *! bLen then ones t SEC else BN.bn_lt_pow2_mask bLen b bs
+
+
+inline_for_extraction noextract
+let rsapss_check_modulus_st (t:limb_t) =
+    modBits:size_t{0 < v modBits /\ bits t * v (blocks modBits (size (bits t))) <= max_size_t}
+  -> n:lbignum t (blocks modBits (size (bits t))) ->
+  Stack (limb t)
   (requires fun h -> live h n)
   (ensures  fun h0 r h1 -> modifies0 h0 h1 /\
     r == LS.rsapss_check_modulus (v modBits) (as_seq h0 n))
 
-[@CInline]
-let rsapss_check_modulus modBits n =
-  let nLen = blocks modBits 64ul in
-  let bits0 = bn_is_odd nLen n in
-  let m0 = u64 0 -. bits0 in
-  let m1 = bn_gt_pow2_mask nLen n (modBits -! 1ul) in
+
+inline_for_extraction noextract
+val rsapss_check_modulus: #t:limb_t -> rsapss_check_modulus_st t
+let rsapss_check_modulus #t modBits n =
+  let nLen = blocks modBits (size (bits t)) in
+  let bits0 = BN.bn_is_odd nLen n in
+  let m0 = uint #t 0 -. bits0 in
+  let m1 = BN.bn_gt_pow2_mask nLen n (modBits -! 1ul) in
   let m2 = bn_check_num_bits modBits n in
   m0 &. (m1 &. m2)
 
 
-val rsapss_check_exponent:
-    eBits:size_t{0 < v eBits /\ 64 * v (blocks eBits 64ul) <= max_size_t}
-  -> e:lbignum (blocks eBits 64ul) ->
-  Stack uint64
+inline_for_extraction noextract
+let rsapss_check_exponent_st (t:limb_t) =
+    eBits:size_t{0 < v eBits /\ bits t * v (blocks eBits (size (bits t))) <= max_size_t}
+  -> e:lbignum t (blocks eBits (size (bits t))) ->
+  Stack (limb t)
   (requires fun h -> live h e)
   (ensures  fun h0 r h1 -> modifies0 h0 h1 /\
     r == LS.rsapss_check_exponent (v eBits) (as_seq h0 e))
 
-[@CInline]
-let rsapss_check_exponent eBits e =
-  let eLen = blocks eBits 64ul in
-  let m0 = bn_is_zero_mask eLen e in
+
+inline_for_extraction noextract
+val rsapss_check_exponent: #t:limb_t -> rsapss_check_exponent_st t
+let rsapss_check_exponent #t eBits e =
+  let eLen = blocks eBits (size (bits t)) in
+  let m0 = BN.bn_is_zero_mask eLen e in
   let m1 = bn_check_num_bits eBits e in
   (lognot m0) &. m1
 
 
 //pkey = [n; r2; e]
 inline_for_extraction noextract
-let rsapss_load_pkey_st =
+let rsapss_load_pkey_st (t:limb_t) =
     modBits:size_t
-  -> eBits:size_t{LS.pkey_len_pre (v modBits) (v eBits)}
+  -> eBits:size_t{LS.pkey_len_pre t (v modBits) (v eBits)}
   -> nb:lbuffer uint8 (blocks modBits 8ul)
   -> eb:lbuffer uint8 (blocks eBits 8ul)
-  -> pkey:lbignum (2ul *! blocks modBits 64ul +! blocks eBits 64ul) ->
+  -> pkey:lbignum t (2ul *! blocks modBits (size (bits t)) +! blocks eBits (size (bits t))) ->
   Stack bool
   (requires fun h ->
     live h nb /\ live h eb /\ live h pkey /\
@@ -87,33 +140,31 @@ let rsapss_load_pkey_st =
    (b, as_seq h1 pkey) == LS.rsapss_load_pkey (v modBits) (v eBits) (as_seq h0 nb) (as_seq h0 eb))
 
 
-val rsapss_load_pkey: rsapss_load_pkey_st
-[@CInline]
-let rsapss_load_pkey modBits eBits nb eb pkey =
+inline_for_extraction noextract
+val rsapss_load_pkey: #t:limb_t -> rsapss_load_pkey_st t
+let rsapss_load_pkey #t modBits eBits nb eb pkey =
   let h0 = ST.get () in
+  [@inline_let] let bits = size (bits t) in
+  [@inline_let] let numb = size (numbytes t) in
   let nbLen = blocks modBits 8ul in
   let ebLen = blocks eBits 8ul in
 
-  let nLen = blocks modBits 64ul in
-  let eLen = blocks eBits 64ul in
+  let nLen = blocks modBits bits in
+  let eLen = blocks eBits bits in
 
-  LS.blocks_bits_lemma (v modBits);
-  LS.blocks_bits_lemma1 (v modBits);
-  assert (0 < v nbLen /\ 8 * v nbLen <= max_size_t);
-  assert (v (blocks nbLen 8ul) == v nLen);
+  LS.blocks_bits_lemma t (v modBits);
+  assert (v (blocks nbLen numb) == v nLen);
 
-  LS.blocks_bits_lemma (v eBits);
-  LS.blocks_bits_lemma1 (v eBits);
-  assert (0 < v ebLen /\ 8 * v ebLen <= max_size_t);
-  assert (v (blocks ebLen 8ul) == v eLen);
+  LS.blocks_bits_lemma t (v eBits);
+  assert (v (blocks ebLen numb) == v eLen);
 
   let n  = sub pkey 0ul nLen in
   let r2 = sub pkey nLen nLen in
   let e  = sub pkey (nLen +! nLen) eLen in
 
-  bn_from_bytes_be nbLen nb n;
-  BM.precomp_r2_mod_n #nLen #(BN.mk_runtime_bn nLen) n r2;
-  bn_from_bytes_be ebLen eb e;
+  BN.bn_from_bytes_be nbLen nb n;
+  BM.bn_precomp_r2_mod_n #t (BN.mk_runtime_bn t nLen) n r2;
+  BN.bn_from_bytes_be ebLen eb e;
   let h1 = ST.get () in
   LSeq.lemma_concat3 (v nLen) (as_seq h1 n)
     (v nLen) (as_seq h1 r2) (v eLen) (as_seq h1 e) (as_seq h1 pkey);
@@ -121,21 +172,21 @@ let rsapss_load_pkey modBits eBits nb eb pkey =
   let m0 = rsapss_check_modulus modBits n in
   let m1 = rsapss_check_exponent eBits e in
   let m = m0 &. m1 in
-  BB.unsafe_bool_of_u64 m
+  BB.unsafe_bool_of_limb #t m
 
 
 #set-options "--z3rlimit 300"
 
 //skey = [pkey; d]
 inline_for_extraction noextract
-let rsapss_load_skey_st =
-    modBits:size_t
+let rsapss_load_skey_st (t:limb_t) =
+     modBits:size_t
   -> eBits:size_t
-  -> dBits:size_t{LS.skey_len_pre (v modBits) (v eBits) (v dBits)}
+  -> dBits:size_t{LS.skey_len_pre t (v modBits) (v eBits) (v dBits)}
   -> nb:lbuffer uint8 (blocks modBits 8ul)
   -> eb:lbuffer uint8 (blocks eBits 8ul)
   -> db:lbuffer uint8 (blocks dBits 8ul)
-  -> skey:lbignum (2ul *! blocks modBits 64ul +! blocks eBits 64ul +! blocks dBits 64ul) ->
+  -> skey:lbignum t (2ul *! blocks modBits (size (bits t)) +! blocks eBits (size (bits t)) +! blocks dBits (size (bits t))) ->
   Stack bool
   (requires fun h ->
     live h nb /\ live h eb /\ live h db /\ live h skey /\
@@ -145,97 +196,97 @@ let rsapss_load_skey_st =
       (as_seq h0 nb) (as_seq h0 eb) (as_seq h0 db))
 
 
-val rsapss_load_skey: rsapss_load_skey_st
-[@CInline]
-let rsapss_load_skey modBits eBits dBits nb eb db skey =
+inline_for_extraction noextract
+val rsapss_load_skey: #t:limb_t -> rsapss_load_skey_st t
+let rsapss_load_skey #t modBits eBits dBits nb eb db skey =
   let h0 = ST.get () in
+  [@inline_let] let bits = size (bits t) in
+  [@inline_let] let numb = size (numbytes t) in
   let nbLen = blocks modBits 8ul in
   let ebLen = blocks eBits 8ul in
   let dbLen = blocks dBits 8ul in
 
-  let nLen = blocks modBits 64ul in
-  let eLen = blocks eBits 64ul in
-  let dLen = blocks dBits 64ul in
+  let nLen = blocks modBits bits in
+  let eLen = blocks eBits bits in
+  let dLen = blocks dBits bits in
 
   let pkeyLen = nLen +! nLen +! eLen in
   let skeyLen = pkeyLen +! eLen in
 
-  LS.blocks_bits_lemma (v dBits);
-  LS.blocks_bits_lemma1 (v dBits);
-  assert (0 < v dbLen /\ 8 * v dbLen <= max_size_t);
-  assert (v (blocks dbLen 8ul) == v dLen);
+  LS.blocks_bits_lemma t (v dBits);
+  assert (v (blocks dbLen numb) == v dLen);
 
   let pkey = sub skey 0ul pkeyLen in
   let d = sub skey pkeyLen dLen in
 
   let b = rsapss_load_pkey modBits eBits nb eb pkey in
-  bn_from_bytes_be dbLen db d;
+  BN.bn_from_bytes_be dbLen db d;
   let h1 = ST.get () in
   LSeq.lemma_concat2 (v pkeyLen) (as_seq h1 pkey) (v dLen) (as_seq h1 d) (as_seq h1 skey);
 
   let m1 = rsapss_check_exponent dBits d in
-  let b1 = b && BB.unsafe_bool_of_u64 m1 in
+  let b1 = b && BB.unsafe_bool_of_limb m1 in
   b1
 
 
 
 inline_for_extraction noextract
-let new_rsapss_load_pkey_st =
+let new_rsapss_load_pkey_st (t:limb_t) =
     r:HS.rid
   -> modBits:size_t{0 < v modBits}
   -> eBits:size_t{0 < v eBits}
   -> nb:lbuffer uint8 (blocks modBits 8ul)
   -> eb:lbuffer uint8 (blocks eBits 8ul) ->
-  ST (B.buffer uint64)
+  ST (B.buffer (limb t))
   (requires fun h -> live h nb /\ live h eb /\
     ST.is_eternal_region r)
   (ensures  fun h0 pkey h1 -> B.(modifies loc_none h0 h1) /\
     not (B.g_is_null pkey) ==> (
-      LS.pkey_len_pre (v modBits) (v eBits) /\
+      LS.pkey_len_pre t (v modBits) (v eBits) /\
       B.(fresh_loc (loc_buffer pkey) h0 h1) /\
       B.(loc_includes (loc_region_only false r) (loc_buffer pkey)) /\
-     (let nLen = blocks modBits 64ul in
-      let eLen = blocks eBits 64ul in
+     (let bits = size (bits t) in
+      let nLen = blocks modBits bits in
+      let eLen = blocks eBits bits in
       let pkeyLen = nLen +! nLen +! eLen in
       B.len pkey == pkeyLen /\
-     (let pkey = pkey <: lbignum pkeyLen in
+     (let pkey = pkey <: lbignum t pkeyLen in
 
       LS.rsapss_load_pkey_post (v modBits) (v eBits)
 	(as_seq h0 nb) (as_seq h0 eb) (as_seq h1 pkey)))))
 
 
 inline_for_extraction noextract
-val new_rsapss_load_pkey: new_rsapss_load_pkey_st
-let new_rsapss_load_pkey r modBits eBits nb eb =
-  let nLen = blocks modBits 64ul in
-  let eLen = blocks eBits 64ul in
+val new_rsapss_load_pkey: #t:limb_t -> new_rsapss_load_pkey_st t
+let new_rsapss_load_pkey #t r modBits eBits nb eb =
+  [@inline_let] let bits = size (bits t) in
+  let nLen = blocks modBits bits in
+  let eLen = blocks eBits bits in
   let pkeyLen = nLen +! nLen +! eLen in
 
-  if not (1ul <. modBits && 0ul <. eBits &&
-    nLen <=. 0xfffffffful /. 128ul && eLen <=. 0xfffffffful /. 64ul &&
-    nLen +! nLen <=. 0xfffffffful -. eLen) then
+  if not (rsapss_check_pkey_len #t modBits eBits) then
    B.null
   else
     let h0 = ST.get () in
-    let pkey = LowStar.Monotonic.Buffer.mmalloc_partial r (u64 0) pkeyLen in
+    let pkey = LowStar.Monotonic.Buffer.mmalloc_partial r (uint #t 0) pkeyLen in
     if B.is_null pkey then
       pkey
     else
       let h1 = ST.get () in
       B.(modifies_only_not_unused_in loc_none h0 h1);
       assert (B.len pkey == pkeyLen);
-      let pkey: Lib.Buffer.buffer Lib.IntTypes.uint64 = pkey in
+      let pkey: Lib.Buffer.buffer (limb t) = pkey in
       assert (B.length pkey == FStar.UInt32.v pkeyLen);
-      let pkey: lbignum pkeyLen = pkey in
+      let pkey: lbignum t pkeyLen = pkey in
       let b = rsapss_load_pkey modBits eBits nb eb pkey in
       let h2 = ST.get () in
       B.(modifies_only_not_unused_in loc_none h0 h2);
-      LS.rsapss_load_pkey_lemma (v modBits) (v eBits) (as_seq h0 nb) (as_seq h0 eb);
+      LS.rsapss_load_pkey_lemma #t (v modBits) (v eBits) (as_seq h0 nb) (as_seq h0 eb);
       if b then pkey else B.null
 
 
 inline_for_extraction noextract
-let new_rsapss_load_skey_st =
+let new_rsapss_load_skey_st (t:limb_t) =
     r:HS.rid
   -> modBits:size_t{0 < v modBits}
   -> eBits:size_t{0 < v eBits}
@@ -243,52 +294,53 @@ let new_rsapss_load_skey_st =
   -> nb:lbuffer uint8 (blocks modBits 8ul)
   -> eb:lbuffer uint8 (blocks eBits 8ul)
   -> db:lbuffer uint8 (blocks dBits 8ul) ->
-  ST (B.buffer uint64)
+  ST (B.buffer (limb t))
   (requires fun h -> live h nb /\ live h eb /\ live h db /\
     ST.is_eternal_region r)
   (ensures  fun h0 skey h1 -> B.(modifies loc_none h0 h1) /\
     not (B.g_is_null skey) ==> (
-      LS.skey_len_pre (v modBits) (v eBits) (v dBits) /\
+      LS.skey_len_pre t (v modBits) (v eBits) (v dBits) /\
       B.(fresh_loc (loc_buffer skey) h0 h1) /\
       B.(loc_includes (loc_region_only false r) (loc_buffer skey)) /\
-     (let nLen = blocks modBits 64ul in
-      let eLen = blocks eBits 64ul in
-      let dLen = blocks dBits 64ul in
+     (let bits = size (bits t) in
+      let nLen = blocks modBits bits in
+      let eLen = blocks eBits bits in
+      let dLen = blocks dBits bits in
       let skeyLen = nLen +! nLen +! eLen +! dLen in
 
       B.len skey == skeyLen /\
-     (let skey = skey <: lbignum skeyLen in
+     (let skey = skey <: lbignum t skeyLen in
       LS.rsapss_load_skey_post (v modBits) (v eBits) (v dBits)
 	(as_seq h0 nb) (as_seq h0 eb) (as_seq h0 db) (as_seq h1 skey)))))
 
 
 inline_for_extraction noextract
-val new_rsapss_load_skey: new_rsapss_load_skey_st
-let new_rsapss_load_skey r modBits eBits dBits nb eb db =
-  let nLen = blocks modBits 64ul in
-  let eLen = blocks eBits 64ul in
-  let dLen = blocks dBits 64ul in
+val new_rsapss_load_skey: #t:limb_t -> new_rsapss_load_skey_st t
+let new_rsapss_load_skey #t r modBits eBits dBits nb eb db =
+  [@inline_let] let bits = size (bits t) in
+  let nLen = blocks modBits bits in
+  let eLen = blocks eBits bits in
+  let dLen = blocks dBits bits in
   let skeyLen = nLen +! nLen +! eLen +! dLen in
 
-  if not (1ul <. modBits && 0ul <. eBits && 0ul <. dBits &&
-    nLen <=. 0xfffffffful /. 128ul && eLen <=. 0xfffffffful /. 64ul && dLen <=. 0xfffffffful /. 64ul &&
-    nLen +! nLen <=. 0xfffffffful -. eLen -. dLen) then
+  if not (rsapss_check_skey_len #t modBits eBits dBits) then
    B.null
-  else
+  else begin
+    assert (LS.skey_len_pre t (v modBits) (v eBits) (v dBits));
     let h0 = ST.get () in
-    let skey = LowStar.Monotonic.Buffer.mmalloc_partial r (u64 0) skeyLen in
+    let skey = LowStar.Monotonic.Buffer.mmalloc_partial r (uint #t 0) skeyLen in
     if B.is_null skey then
       skey
     else
       let h1 = ST.get () in
       B.(modifies_only_not_unused_in loc_none h0 h1);
       assert (B.len skey == skeyLen);
-      let skey: Lib.Buffer.buffer Lib.IntTypes.uint64 = skey in
+      let skey: Lib.Buffer.buffer (limb t) = skey in
       assert (B.length skey == FStar.UInt32.v skeyLen);
-      let skey: lbignum skeyLen = skey in
-      let b = rsapss_load_skey modBits eBits dBits nb eb db skey in
+      let skey: lbignum t skeyLen = skey in
+      let b = rsapss_load_skey #t modBits eBits dBits nb eb db skey in
       let h2 = ST.get () in
       B.(modifies_only_not_unused_in loc_none h0 h2);
-      LS.rsapss_load_skey_lemma (v modBits) (v eBits) (v dBits)
+      LS.rsapss_load_skey_lemma #t (v modBits) (v eBits) (v dBits)
 	(as_seq h0 nb) (as_seq h0 eb) (as_seq h0 db);
-      if b then skey else B.null
+      if b then skey else B.null end
