code/rsapss/Hacl.RSAPSS.fst
@@ -1,33 +1,48 @@
 module Hacl.RSAPSS
 
+open Lib.IntTypes
+
 module S = Spec.RSAPSS
 module Hash = Spec.Agile.Hash
 
 module IR = Hacl.Impl.RSAPSS
 module IK = Hacl.Impl.RSAPSS.Keys
 
+module BN = Hacl.Bignum
+module BE = Hacl.Bignum.Exponentiation
+module BD = Hacl.Bignum.Definitions
+
 #reset-options "--z3rlimit 50 --fuel 0 --ifuel 0"
 
-val rsapss_sign: a:Hash.algorithm{S.hash_is_supported a} -> IR.rsapss_sign_st a
+val rsapss_sign: IR.rsapss_sign_st U64
 let rsapss_sign a modBits eBits dBits skey sLen salt msgLen msg sgnt =
-  IR.rsapss_sign a modBits eBits dBits skey sLen salt msgLen msg sgnt
+  [@inline_let] let ke = BE.mk_runtime_exp_uint64 (BD.blocks modBits 64ul) in
+  IR.rsapss_sign ke a modBits eBits dBits skey sLen salt msgLen msg sgnt
 
-val rsapss_verify: a:Hash.algorithm{S.hash_is_supported a} -> IR.rsapss_verify_st a
+
+val rsapss_verify: IR.rsapss_verify_st U64
 let rsapss_verify a modBits eBits pkey sLen k sgnt msgLen msg =
-  IR.rsapss_verify a modBits eBits pkey sLen k sgnt msgLen msg
+  [@inline_let] let ke = BE.mk_runtime_exp_uint64 (BD.blocks modBits 64ul) in
+  IR.rsapss_verify ke a modBits eBits pkey sLen k sgnt msgLen msg
 
-val new_rsapss_load_pkey: IK.new_rsapss_load_pkey_st
+
+val new_rsapss_load_pkey: IK.new_rsapss_load_pkey_st U64
 let new_rsapss_load_pkey r modBits eBits nb eb =
   IK.new_rsapss_load_pkey r modBits eBits nb eb
 
-val new_rsapss_load_skey: IK.new_rsapss_load_skey_st
+
+val new_rsapss_load_skey: IK.new_rsapss_load_skey_st U64
 let new_rsapss_load_skey r modBits eBits dBits nb eb db =
   IK.new_rsapss_load_skey r modBits eBits dBits nb eb db
 
-val rsapss_skey_sign: a:Hash.algorithm{S.hash_is_supported a} -> IR.rsapss_skey_sign_st a
-let rsapss_skey_sign a modBits eBits dBits nb eb db sLen salt msgLen msg sgnt =
-  IR.rsapss_skey_sign a modBits eBits dBits nb eb db sLen salt msgLen msg sgnt
 
-val rsapss_pkey_verify: a:Hash.algorithm{S.hash_is_supported a} -> IR.rsapss_pkey_verify_st a
+val rsapss_skey_sign: IR.rsapss_skey_sign_st U64
+let rsapss_skey_sign a modBits eBits dBits nb eb db sLen salt msgLen msg sgnt =
+  [@inline_let] let ke = BE.mk_runtime_exp_uint64 (BD.blocks modBits 64ul) in
+  IR.rsapss_skey_sign #U64 ke a modBits eBits dBits nb eb db sLen salt msgLen msg sgnt
+
+
+val rsapss_pkey_verify: IR.rsapss_pkey_verify_st U64
 let rsapss_pkey_verify a modBits eBits nb eb sLen k sgnt msgLen msg =
-  IR.rsapss_pkey_verify a modBits eBits nb eb sLen k sgnt msgLen msg
+  [@inline_let] let ke = BE.mk_runtime_exp_uint64 (BD.blocks modBits 64ul) in
+  IR.rsapss_pkey_verify #U64 ke a modBits eBits nb eb sLen k sgnt msgLen msg
