code/rsapss/Hacl.Spec.RSAPSS.fst
@@ -17,34 +17,25 @@ module Hash = Spec.Agile.Hash
 
 #reset-options "--z3rlimit 50 --fuel 0 --ifuel 0"
 
-val em_blocks_lt_max_size_t: modBits:size_pos{1 < modBits} -> Lemma
-  (requires 128 * blocks modBits 64 <= max_size_t)
-  (ensures  8 * blocks (blocks (modBits - 1) 8) 8 <= max_size_t)
-let em_blocks_lt_max_size_t modBits = ()
-  // let r = 8 * blocks (blocks (modBits - 1) 8) 8 in
-  // calc (==) {
-  //   r;
-  //   (==) { }
-  //   8 * (((modBits - 2) / 8) / 8 + 1);
-  //   (==) { Math.Lemmas.division_multiplication_lemma (modBits - 2) 8 8 }
-  //   8 * ((modBits - 2) / 64 + 1);
-  //   (==) { }
-  //   8 * blocks (modBits - 1) 64;
-  //   }
+val blocks_bits_lemma: t:limb_t -> bs:size_pos ->
+  Lemma (blocks (blocks bs 8) (numbytes t) == blocks bs (bits t))
+let blocks_bits_lemma t bs = ()
 
-val blocks_bits_lemma: bits:size_pos ->
-  Lemma (blocks (blocks bits 8) 8 == blocks bits 64)
-let blocks_bits_lemma bits = ()
 
-val blocks_bits_lemma1: bits:size_pos{64 * blocks bits 64 <= max_size_t} ->
-  Lemma (8 * blocks bits 8 <= max_size_t)
-let blocks_bits_lemma1 bits = ()
+val bn_lt_pow2: #t:limb_t -> modBits:size_pos{1 < modBits} -> m:lbignum t (blocks modBits (bits t)) -> bool
+let bn_lt_pow2 #t modBits m =
+  if (modBits - 1) % 8 <> 0 then true
+  else BB.unsafe_bool_of_limb0 (bn_get_ith_bit m (modBits - 1))
 
-val bn_eval_lt_pow2_modBits: modBits:size_pos{1 < modBits} -> m:lbignum (blocks modBits 64) -> Lemma
+
+val bn_eval_lt_pow2_modBits:
+    #t:limb_t
+  -> modBits:size_pos{1 < modBits}
+  -> m:lbignum t (blocks modBits (bits t)) -> Lemma
   (requires bn_v m < pow2 modBits)
   (ensures  bn_v m == (bn_v m / pow2 (modBits - 1) % 2) * pow2 (modBits - 1) + bn_v m % pow2 (modBits - 1))
 
-let bn_eval_lt_pow2_modBits modBits m =
+let bn_eval_lt_pow2_modBits #t modBits m =
   calc (==) {
     bn_v m;
     (==) { Math.Lemmas.euclidean_division_definition (bn_v m) (pow2 (modBits - 1)) }
@@ -57,21 +48,16 @@ let bn_eval_lt_pow2_modBits modBits m =
     (bn_v m / pow2 (modBits - 1) % 2) * pow2 (modBits - 1) + bn_v m % pow2 (modBits - 1);
     }
 
-val bn_lt_pow2: modBits:size_pos{1 < modBits} -> m:lbignum (blocks modBits 64) -> bool
-let bn_lt_pow2 modBits m =
-  if (modBits - 1) % 8 <> 0 then true
-  else FStar.UInt64.(Lib.RawIntTypes.u64_to_UInt64 (bn_get_ith_bit m (modBits - 1)) =^ 0uL)
 
-val bn_lt_pow2_lemma: modBits:size_pos{1 < modBits} -> m:lbignum (blocks modBits 64) -> Lemma
+val bn_lt_pow2_lemma: #t:limb_t -> modBits:size_pos{1 < modBits} -> m:lbignum t (blocks modBits (bits t)) -> Lemma
   (requires bn_v m < pow2 modBits)
   (ensures  bn_lt_pow2 modBits m == (bn_v m < pow2 (8 * blocks (modBits - 1) 8)))
 
-let bn_lt_pow2_lemma modBits m =
+let bn_lt_pow2_lemma #t modBits m =
   let k = blocks modBits 8 in
   let emLen = blocks (modBits - 1) 8 in
-  let mLen = blocks emLen 8 in
-  let nLen = blocks k 8 in
-  assert (nLen == blocks modBits 64);
+  let nLen = blocks k (numbytes t) in
+  assert (nLen == blocks modBits (bits t));
 
   if (modBits - 1) % 8 <> 0 then Math.Lemmas.pow2_le_compat (8 * emLen) modBits
   else begin
@@ -81,68 +67,73 @@ let bn_lt_pow2_lemma modBits m =
     assert (8 * emLen == modBits - 1);
 
     bn_eval_lt_pow2_modBits modBits m;
-    let r = FStar.UInt64.(Lib.RawIntTypes.u64_to_UInt64 (bn_get_ith_bit m (modBits - 1)) =^ 0uL) in
     bn_get_ith_bit_lemma m (modBits - 1) end
 
 
-val bn_eval_sub: modBits:size_pos{1 < modBits} -> m:lbignum (blocks modBits 64) -> Lemma
+val bn_eval_sub: #t:limb_t -> modBits:size_pos{1 < modBits} -> m:lbignum t (blocks modBits (bits t)) -> Lemma
   (requires bn_v m < pow2 (8 * blocks (modBits - 1) 8))
-  (ensures  bn_v m == bn_v (sub m 0 (blocks (blocks (modBits - 1) 8) 8)))
+  (ensures  bn_v m == bn_v (sub m 0 (blocks (blocks (modBits - 1) 8) (numbytes t))))
 
-let bn_eval_sub modBits m =
+let bn_eval_sub #t modBits m =
   let emLen = blocks (modBits - 1) 8 in
-  let mLen = blocks emLen 8 in
-  let nLen = blocks modBits 64 in
+  let mLen = blocks emLen (numbytes t) in
+  let nLen = blocks modBits (bits t) in
   assert (bn_v m < pow2 (8 * emLen));
   let m1 = sub m 0 mLen in
   bn_eval_split_i m mLen;
-  assert (bn_v m == bn_v m1 + pow2 (64 * mLen) * bn_v (slice m mLen nLen));
+  assert (bn_v m == bn_v m1 + pow2 (bits t * mLen) * bn_v (slice m mLen nLen));
   bn_eval_bound m1 mLen;
-  assert (bn_v m1 < pow2 (64 * mLen));
-  Math.Lemmas.pow2_le_compat (64 * mLen) (8 * emLen)
+  assert (bn_v m1 < pow2 (bits t * mLen));
+  Math.Lemmas.pow2_le_compat (bits t * mLen) (8 * emLen)
 
 
-let pkey_len_pre (modBits:size_nat) (eBits:size_nat) =
+let pkey_len_pre (t:limb_t) (modBits:size_nat) (eBits:size_nat) =
+  let bits = bits t in
   1 < modBits /\ 0 < eBits /\
-  128 * blocks modBits 64 <= max_size_t /\
-  64 * blocks eBits 64 <= max_size_t /\
-  2 * blocks modBits 64 + blocks eBits 64 <= max_size_t
+  2 * bits * blocks modBits bits <= max_size_t /\
+  bits * blocks eBits bits <= max_size_t /\
+  2 * blocks modBits bits + blocks eBits bits <= max_size_t
 
 
-let skey_len_pre (modBits:size_nat) (eBits:size_nat) (dBits:size_nat) =
-  pkey_len_pre modBits eBits /\
-  0 < dBits /\ 64 * blocks dBits 64 <= max_size_t /\
-  2 * blocks modBits 64 + blocks eBits 64 + blocks dBits 64 <= max_size_t
+let skey_len_pre (t:limb_t) (modBits:size_nat) (eBits:size_nat) (dBits:size_nat) =
+  let bits = bits t in
+  pkey_len_pre t modBits eBits /\
+  0 < dBits /\ bits * blocks dBits bits <= max_size_t /\
+  2 * blocks modBits bits + blocks eBits bits + blocks dBits bits <= max_size_t
 
 
 val rsapss_pkey_pre:
-    modBits:size_nat
-  -> eBits:size_nat{pkey_len_pre modBits eBits}
-  -> pkey:lbignum (2 * blocks modBits 64 + blocks eBits 64) -> Type0
+    #t:limb_t
+  -> modBits:size_nat
+  -> eBits:size_nat{pkey_len_pre t modBits eBits}
+  -> pkey:lbignum t (2 * blocks modBits (bits t) + blocks eBits (bits t)) -> Type0
 
-let rsapss_pkey_pre modBits eBits pkey =
-  let nLen = blocks modBits 64 in
-  let eLen = blocks eBits 64 in
+let rsapss_pkey_pre #t modBits eBits pkey =
+  let bits = bits t in
+  let nLen = blocks modBits bits in
+  let eLen = blocks eBits bits in
 
   let n  = sub pkey 0 nLen in
   let r2 = sub pkey nLen nLen in
   let e = sub pkey (nLen + nLen) eLen in
-  r2 == SM.precomp_r2_mod_n n /\
+  r2 == SM.bn_precomp_r2_mod_n n /\
   bn_v n % 2 = 1 /\
   pow2 (modBits - 1) < bn_v n /\ bn_v n < pow2 modBits /\
   0 < bn_v e /\ bn_v e < pow2 eBits
 
 
 val rsapss_skey_pre:
-    modBits:size_nat
+    #t:limb_t
+  -> modBits:size_nat
   -> eBits:size_nat
-  -> dBits:size_nat{skey_len_pre modBits eBits dBits}
-  -> skey:lbignum (2 * blocks modBits 64 + blocks eBits 64 + blocks dBits 64) -> Type0
+  -> dBits:size_nat{skey_len_pre t modBits eBits dBits}
+  -> skey:lbignum t (2 * blocks modBits (bits t) + blocks eBits (bits t) + blocks dBits (bits t)) -> Type0
 
-let rsapss_skey_pre modBits eBits dBits skey =
-  let nLen = blocks modBits 64 in
-  let eLen = blocks eBits 64 in
-  let dLen = blocks dBits 64 in
+let rsapss_skey_pre #t modBits eBits dBits skey =
+  let bits = bits t in
+  let nLen = blocks modBits bits in
+  let eLen = blocks eBits bits in
+  let dLen = blocks dBits bits in
   let pkeyLen = nLen + nLen + eLen in
 
   let pkey = sub skey 0 pkeyLen in
@@ -152,31 +143,33 @@ let rsapss_skey_pre modBits eBits dBits skey =
 
 
 val rsapss_sign_pre:
-    a:Hash.algorithm{S.hash_is_supported a}
+    #t:limb_t
+  -> a:Hash.algorithm{S.hash_is_supported a}
   -> modBits:size_nat
   -> eBits:size_nat
-  -> dBits:size_nat{skey_len_pre modBits eBits dBits}
-  -> skey:lbignum (2 * blocks modBits 64 + blocks eBits 64 + blocks dBits 64)
+  -> dBits:size_nat{skey_len_pre t modBits eBits dBits}
+  -> skey:lbignum t (2 * blocks modBits (bits t) + blocks eBits (bits t) + blocks dBits (bits t))
   -> sLen:size_nat
   -> salt:lseq uint8 sLen
   -> msgLen:nat
   -> msg:seq uint8{length msg == msgLen} -> Type0
 
-let rsapss_sign_pre a modBits eBits dBits skey sLen salt msgLen msg =
+let rsapss_sign_pre #t a modBits eBits dBits skey sLen salt msgLen msg =
   sLen + Hash.hash_length a + 8 <= max_size_t /\
   sLen + Hash.hash_length a + 8 <= Hash.max_input_length a /\
-  sLen + Hash.hash_length a + 2 <= (blocks (modBits - 1) 8) /\
+  sLen + Hash.hash_length a + 2 <= blocks (modBits - 1) 8 /\
   msgLen <= Hash.max_input_length a /\
 
   rsapss_skey_pre modBits eBits dBits skey
 
 
 val rsapss_sign_post:
-    a:Hash.algorithm{S.hash_is_supported a}
+    #t:limb_t
+  -> a:Hash.algorithm{S.hash_is_supported a}
   -> modBits:size_nat
   -> eBits:size_nat
-  -> dBits:size_nat{skey_len_pre modBits eBits dBits}
-  -> skey:lbignum (2 * blocks modBits 64 + blocks eBits 64 + blocks dBits 64)
+  -> dBits:size_nat{skey_len_pre t modBits eBits dBits}
+  -> skey:lbignum t (2 * blocks modBits (bits t) + blocks eBits (bits t) + blocks dBits (bits t))
   -> sLen:size_nat
   -> salt:lseq uint8 sLen
   -> msgLen:nat
@@ -184,11 +177,12 @@ val rsapss_sign_post:
   -> eq_m:bool
   -> sgnt:lseq uint8 (blocks modBits 8) -> Type0
 
-let rsapss_sign_post a modBits eBits dBits skey sLen salt msgLen msg eq_m sgnt =
+let rsapss_sign_post #t a modBits eBits dBits skey sLen salt msgLen msg eq_m sgnt =
   rsapss_sign_pre a modBits eBits dBits skey sLen salt msgLen msg /\
- (let nLen = blocks modBits 64 in
-  let eLen = blocks eBits 64 in
-  let dLen = blocks dBits 64 in
+ (let bits = bits t in
+  let nLen = blocks modBits bits in
+  let eLen = blocks eBits bits in
+  let dLen = blocks dBits bits in
 
   let n = bn_v (sub skey 0 nLen) in
   let e = bn_v (sub skey (nLen + nLen) eLen) in
@@ -200,11 +194,12 @@ let rsapss_sign_post a modBits eBits dBits skey sLen salt msgLen msg eq_m sgnt =
 
 
 val rsapss_sign_post1:
-    a:Hash.algorithm{S.hash_is_supported a}
+    #t:limb_t
+  -> a:Hash.algorithm{S.hash_is_supported a}
   -> modBits:size_nat
   -> eBits:size_nat
-  -> dBits:size_nat{skey_len_pre modBits eBits dBits}
-  -> skey:lbignum (2 * blocks modBits 64 + blocks eBits 64 + blocks dBits 64)
+  -> dBits:size_nat{skey_len_pre t modBits eBits dBits}
+  -> skey:lbignum t (2 * blocks modBits (bits t) + blocks eBits (bits t) + blocks dBits (bits t))
   -> sLen:size_nat
   -> salt:lseq uint8 sLen
   -> msgLen:nat
@@ -212,11 +207,12 @@ val rsapss_sign_post1:
   -> eq_m:bool
   -> sgnt:lseq uint8 (blocks modBits 8) -> Type0
 
-let rsapss_sign_post1 a modBits eBits dBits skey sLen salt msgLen msg eq_m sgnt =
+let rsapss_sign_post1 #t a modBits eBits dBits skey sLen salt msgLen msg eq_m sgnt =
   rsapss_skey_pre modBits eBits dBits skey /\
- (let nLen = blocks modBits 64 in
-  let eLen = blocks eBits 64 in
-  let dLen = blocks dBits 64 in
+ (let bits = bits t in
+  let nLen = blocks modBits bits in
+  let eLen = blocks eBits bits in
+  let dLen = blocks dBits bits in
 
   let n = bn_v (sub skey 0 nLen) in
   let e = bn_v (sub skey (nLen + nLen) eLen) in
@@ -228,15 +224,16 @@ let rsapss_sign_post1 a modBits eBits dBits skey sLen salt msgLen msg eq_m sgnt 
 
 
 val rsapss_verify_pre:
-    a:Hash.algorithm{S.hash_is_supported a}
+    #t:limb_t
+  -> a:Hash.algorithm{S.hash_is_supported a}
   -> modBits:size_nat
-  -> eBits:size_nat{pkey_len_pre modBits eBits}
-  -> pkey:lbignum (2 * blocks modBits 64 + blocks eBits 64)
+  -> eBits:size_nat{pkey_len_pre t modBits eBits}
+  -> pkey:lbignum t (2 * blocks modBits (bits t) + blocks eBits (bits t))
   -> sLen:size_nat //saltLen
   -> msgLen:nat
   -> msg:seq uint8{length msg == msgLen} -> Type0
 
-let rsapss_verify_pre a modBits eBits pkey sLen msgLen msg =
+let rsapss_verify_pre #t a modBits eBits pkey sLen msgLen msg =
   sLen + Hash.hash_length a + 8 <= max_size_t /\
   sLen + Hash.hash_length a + 8 <= Hash.max_input_length a /\
   msgLen <= Hash.max_input_length a /\
@@ -245,20 +242,22 @@ let rsapss_verify_pre a modBits eBits pkey sLen msgLen msg =
 
 
 val rsapss_verify_post:
-    a:Hash.algorithm{S.hash_is_supported a}
+    #t:limb_t
+  -> a:Hash.algorithm{S.hash_is_supported a}
   -> modBits:size_nat
-  -> eBits:size_nat{pkey_len_pre modBits eBits}
-  -> pkey:lbignum (2 * blocks modBits 64 + blocks eBits 64)
+  -> eBits:size_nat{pkey_len_pre t modBits eBits}
+  -> pkey:lbignum t (2 * blocks modBits (bits t) + blocks eBits (bits t))
   -> sLen:size_nat //saltLen
   -> sgnt:lseq uint8 (blocks modBits 8)
   -> msgLen:nat
   -> msg:seq uint8{length msg == msgLen}
   -> verify:bool -> Type0
 
-let rsapss_verify_post a modBits eBits pkey sLen sgnt msgLen msg verify =
+let rsapss_verify_post #t a modBits eBits pkey sLen sgnt msgLen msg verify =
   rsapss_verify_pre a modBits eBits pkey sLen msgLen msg /\
- (let nLen = blocks modBits 64 in
-  let eLen = blocks eBits 64 in
+ (let bits = bits t in
+  let nLen = blocks modBits bits in
+  let eLen = blocks eBits bits in
 
   let n = bn_v (sub pkey 0 nLen) in
   let e = bn_v (sub pkey (nLen + nLen) eLen) in
@@ -267,10 +266,11 @@ let rsapss_verify_post a modBits eBits pkey sLen sgnt msgLen msg verify =
 
 
 val rsapss_verify_post1:
-    a:Hash.algorithm{S.hash_is_supported a}
+    #t:limb_t
+  -> a:Hash.algorithm{S.hash_is_supported a}
   -> modBits:size_nat
-  -> eBits:size_nat{pkey_len_pre modBits eBits}
-  -> pkey:lbignum (2 * blocks modBits 64 + blocks eBits 64)
+  -> eBits:size_nat{pkey_len_pre t modBits eBits}
+  -> pkey:lbignum t (2 * blocks modBits (bits t) + blocks eBits (bits t))
   -> sLen:size_nat //saltLen
   -> k:size_nat
   -> sgnt:lseq uint8 k
@@ -278,10 +278,11 @@ val rsapss_verify_post1:
   -> msg:seq uint8{length msg == msgLen}
   -> verify:bool -> Type0
 
-let rsapss_verify_post1 a modBits eBits pkey sLen k sgnt msgLen msg verify =
+let rsapss_verify_post1 #t a modBits eBits pkey sLen k sgnt msgLen msg verify =
   rsapss_pkey_pre modBits eBits pkey /\
- (let nLen = blocks modBits 64 in
-  let eLen = blocks eBits 64 in
+ (let bits = bits t in
+  let nLen = blocks modBits bits in
+  let eLen = blocks eBits bits in
 
   let n = bn_v (sub pkey 0 nLen) in
   let e = bn_v (sub pkey (nLen + nLen) eLen) in
@@ -290,11 +291,12 @@ let rsapss_verify_post1 a modBits eBits pkey sLen k sgnt msgLen msg verify =
 
 
 val rsapss_sign_:
-    a:Hash.algorithm{S.hash_is_supported a}
+    #t:limb_t
+  -> a:Hash.algorithm{S.hash_is_supported a}
   -> modBits:size_nat
   -> eBits:size_nat
-  -> dBits:size_nat{skey_len_pre modBits eBits dBits}
-  -> skey:lbignum (2 * blocks modBits 64 + blocks eBits 64 + blocks dBits 64)
+  -> dBits:size_nat{skey_len_pre t modBits eBits dBits}
+  -> skey:lbignum t (2 * blocks modBits (bits t) + blocks eBits (bits t) + blocks dBits (bits t))
   -> sLen:size_nat
   -> salt:lseq uint8 sLen
   -> msgLen:nat
@@ -303,10 +305,12 @@ val rsapss_sign_:
   (requires rsapss_sign_pre a modBits eBits dBits skey sLen salt msgLen msg)
   (ensures  fun sgnt -> True)
 
-let rsapss_sign_ a modBits eBits dBits skey sLen salt msgLen msg =
-  let nLen = blocks modBits 64 in
-  let eLen = blocks eBits 64 in
-  let dLen = blocks dBits 64 in
+let rsapss_sign_ #t a modBits eBits dBits skey sLen salt msgLen msg =
+  let bits = bits t in
+  let numb = numbytes t in
+  let nLen = blocks modBits bits in
+  let eLen = blocks eBits bits in
+  let dLen = blocks dBits bits in
 
   let n  = sub skey 0 nLen in
   let r2 = sub skey nLen nLen in
@@ -318,29 +322,30 @@ let rsapss_sign_ a modBits eBits dBits skey sLen salt msgLen msg =
   let emLen = blocks emBits 8 in
 
   let em = S.pss_encode a sLen salt msgLen msg emBits in
-  em_blocks_lt_max_size_t modBits;
-  assert (8 * blocks emLen 8 <= max_size_t);
-  let emNat = bn_from_bytes_be emLen em in
-  let m = create nLen (u64 0) in
-  let m = update_sub m 0 (blocks emLen 8) emNat in
+  blocks_bits_lemma t emBits;
+  assert (blocks emLen numb == blocks emBits bits);
+  let emNat = bn_from_bytes_be #t emLen em in
+  let m = create nLen (uint #t 0) in
+  let m = update_sub m 0 (blocks emLen numb) emNat in
 
   let s = bn_mod_exp_mont_ladder_precompr2 nLen n m dBits d r2 in
   let m' = bn_mod_exp_precompr2 nLen n s eBits e r2 in
   let eq_m = bn_eq_mask m m' in
   let s = map (logand eq_m) s in
 
-  blocks_bits_lemma modBits;
-  assert (blocks k 8 == nLen);
+  blocks_bits_lemma t modBits;
+  assert (blocks k numb == nLen);
   let sgnt = bn_to_bytes_be k s in
-  BB.unsafe_bool_of_u64 eq_m, sgnt
+  BB.unsafe_bool_of_limb eq_m, sgnt
 
 
 val rsapss_sign_lemma:
-    a:Hash.algorithm{S.hash_is_supported a}
+    #t:limb_t
+  -> a:Hash.algorithm{S.hash_is_supported a}
   -> modBits:size_nat
   -> eBits:size_nat
-  -> dBits:size_nat{skey_len_pre modBits eBits dBits}
-  -> skey:lbignum (2 * blocks modBits 64 + blocks eBits 64 + blocks dBits 64)
+  -> dBits:size_nat{skey_len_pre t modBits eBits dBits}
+  -> skey:lbignum t (2 * blocks modBits (bits t) + blocks eBits (bits t) + blocks dBits (bits t))
   -> sLen:size_nat
   -> salt:lseq uint8 sLen
   -> msgLen:nat
@@ -351,10 +356,12 @@ val rsapss_sign_lemma:
    (let eq_m, s = rsapss_sign_ a modBits eBits dBits skey sLen salt msgLen msg in
     rsapss_sign_post a modBits eBits dBits skey sLen salt msgLen msg eq_m s))
 
-let rsapss_sign_lemma a modBits eBits dBits skey sLen salt msgLen msg =
-  let nLen = blocks modBits 64 in
-  let eLen = blocks eBits 64 in
-  let dLen = blocks dBits 64 in
+let rsapss_sign_lemma #t a modBits eBits dBits skey sLen salt msgLen msg =
+  let bits = bits t in
+  let numb = numbytes t in
+  let nLen = blocks modBits bits in
+  let eLen = blocks eBits bits in
+  let dLen = blocks dBits bits in
 
   let n  = sub skey 0 nLen in
   let r2 = sub skey nLen nLen in
@@ -366,21 +373,21 @@ let rsapss_sign_lemma a modBits eBits dBits skey sLen salt msgLen msg =
   let emLen = blocks emBits 8 in
 
   let em = S.pss_encode a sLen salt msgLen msg emBits in
-  em_blocks_lt_max_size_t modBits;
-  assert (8 * blocks emLen 8 <= max_size_t);
+  blocks_bits_lemma t emBits;
+  assert (blocks emLen numb == blocks emBits bits);
 
   let emNat = bn_from_bytes_be emLen em in
-  let m = create nLen (u64 0) in
-  let m = update_sub m 0 (blocks emLen 8) emNat in
-  bn_eval_update_sub (blocks emLen 8) emNat nLen;
+  let m = create nLen (uint #t 0) in
+  let m = update_sub m 0 (blocks emLen numb) emNat in
+  bn_eval_update_sub (blocks emLen numb) emNat nLen;
   assert (bn_v m == bn_v emNat);
-  bn_from_bytes_be_lemma emLen em;
+  bn_from_bytes_be_lemma #t emLen em;
   S.os2ip_lemma emBits em;
 
   assert (bn_v m < bn_v n);
   let s = bn_mod_exp_mont_ladder_precompr2 nLen n m dBits d r2 in
-  Math.Lemmas.pow2_le_compat (64 * nLen) modBits;
-  SM.precomp_r2_mod_n_lemma n;
+  Math.Lemmas.pow2_le_compat (bits * nLen) modBits;
+  SM.bn_precomp_r2_mod_n_lemma n;
   bn_mod_exp_mont_ladder_precompr2_lemma nLen n m dBits d r2;
 
   let m' = bn_mod_exp_precompr2 nLen n s eBits e r2 in
@@ -392,8 +399,8 @@ let rsapss_sign_lemma a modBits eBits dBits skey sLen salt msgLen msg =
   let s' = map (logand eq_m) s in
   bn_mask_lemma s eq_m;
 
-  blocks_bits_lemma modBits;
-  assert (blocks k 8 == nLen);
+  blocks_bits_lemma t modBits;
+  assert (blocks k numb == nLen);
   Math.Lemmas.pow2_le_compat (8 * k) modBits;
   assert (bn_v s' < pow2 (8 * k));
   let sgnt = bn_to_bytes_be k s' in
@@ -401,11 +408,12 @@ let rsapss_sign_lemma a modBits eBits dBits skey sLen salt msgLen msg =
 
 
 val rsapss_sign:
-    a:Hash.algorithm{S.hash_is_supported a}
+    #t:limb_t
+  -> a:Hash.algorithm{S.hash_is_supported a}
   -> modBits:size_nat
   -> eBits:size_nat
-  -> dBits:size_nat{skey_len_pre modBits eBits dBits}
-  -> skey:lbignum (2 * blocks modBits 64 + blocks eBits 64 + blocks dBits 64)
+  -> dBits:size_nat{skey_len_pre t modBits eBits dBits}
+  -> skey:lbignum t (2 * blocks modBits (bits t) + blocks eBits (bits t) + blocks dBits (bits t))
   -> sLen:size_nat
   -> salt:lseq uint8 sLen
   -> msgLen:nat
@@ -416,7 +424,7 @@ val rsapss_sign:
   (ensures  fun (b, sgnt) ->
     rsapss_sign_post1 a modBits eBits dBits skey sLen salt msgLen msg b sgnt)
 
-let rsapss_sign a modBits eBits dBits skey sLen salt msgLen msg sgnt =
+let rsapss_sign #t a modBits eBits dBits skey sLen salt msgLen msg sgnt =
   let hLen = Hash.hash_length a in
   Math.Lemmas.pow2_lt_compat 61 32;
   Math.Lemmas.pow2_lt_compat 125 32;
@@ -435,10 +443,11 @@ let rsapss_sign a modBits eBits dBits skey sLen salt msgLen msg sgnt =
 
 
 val rsapss_verify_:
-    a:Hash.algorithm{S.hash_is_supported a}
+    #t:limb_t
+  -> a:Hash.algorithm{S.hash_is_supported a}
   -> modBits:size_nat
-  -> eBits:size_nat{pkey_len_pre modBits eBits}
-  -> pkey:lbignum (2 * blocks modBits 64 + blocks eBits 64)
+  -> eBits:size_nat{pkey_len_pre t modBits eBits}
+  -> pkey:lbignum t (2 * blocks modBits (bits t) + blocks eBits (bits t))
   -> sLen:size_nat //saltLen
   -> sgnt:lseq uint8 (blocks modBits 8)
   -> msgLen:nat
@@ -447,9 +456,11 @@ val rsapss_verify_:
   (requires rsapss_verify_pre a modBits eBits pkey sLen msgLen msg)
   (ensures  fun r -> True)
 
-let rsapss_verify_ a modBits eBits pkey sLen sgnt msgLen msg =
-  let nLen = blocks modBits 64 in
-  let eLen = blocks eBits 64 in
+let rsapss_verify_ #t a modBits eBits pkey sLen sgnt msgLen msg =
+  let bits = bits t in
+  let numb = numbytes t in
+  let nLen = blocks modBits bits in
+  let eLen = blocks eBits bits in
 
   let n  = sub pkey 0 nLen in
   let r2 = sub pkey nLen nLen in
@@ -459,18 +470,18 @@ let rsapss_verify_ a modBits eBits pkey sLen sgnt msgLen msg =
   let emBits = modBits - 1 in
   let emLen = blocks emBits 8 in
 
-  blocks_bits_lemma modBits;
-  assert (blocks k 8 == nLen);
+  blocks_bits_lemma t modBits;
+  assert (blocks k numb == nLen);
   let s = bn_from_bytes_be k sgnt in
 
   let mask = bn_lt_mask s n in
-  if BB.unsafe_bool_of_u64 mask then begin
+  if BB.unsafe_bool_of_limb mask then begin
     let m = bn_mod_exp_precompr2 nLen n s eBits e r2 in
-    em_blocks_lt_max_size_t modBits;
-    assert (8 * blocks emLen 8 <= max_size_t);
+    blocks_bits_lemma t emBits;
+    assert (blocks emLen numb == blocks emBits bits);
 
     if bn_lt_pow2 modBits m then begin
-      let m1 = sub m 0 (blocks emLen 8) in
+      let m1 = sub m 0 (blocks emLen numb) in
       let em = bn_to_bytes_be emLen m1 in
       S.pss_verify a sLen msgLen msg emBits em end
     else false end
@@ -478,10 +489,11 @@ let rsapss_verify_ a modBits eBits pkey sLen sgnt msgLen msg =
 
 
 val rsapss_verify_lemma:
-    a:Hash.algorithm{S.hash_is_supported a}
+    #t:limb_t
+  -> a:Hash.algorithm{S.hash_is_supported a}
   -> modBits:size_nat
-  -> eBits:size_nat{pkey_len_pre modBits eBits}
-  -> pkey:lbignum (2 * blocks modBits 64 + blocks eBits 64)
+  -> eBits:size_nat{pkey_len_pre t modBits eBits}
+  -> pkey:lbignum t (2 * blocks modBits (bits t) + blocks eBits (bits t))
   -> sLen:size_nat //saltLen
   -> sgnt:lseq uint8 (blocks modBits 8)
   -> msgLen:nat
@@ -492,9 +504,11 @@ val rsapss_verify_lemma:
     rsapss_verify_post a modBits eBits pkey sLen sgnt msgLen msg
       (rsapss_verify_ a modBits eBits pkey sLen sgnt msgLen msg))
 
-let rsapss_verify_lemma a modBits eBits pkey sLen sgnt msgLen msg =
-  let nLen = blocks modBits 64 in
-  let eLen = blocks eBits 64 in
+let rsapss_verify_lemma #t a modBits eBits pkey sLen sgnt msgLen msg =
+  let bits = bits t in
+  let numb = numbytes t in
+  let nLen = blocks modBits bits in
+  let eLen = blocks eBits bits in
 
   let n  = sub pkey 0 nLen in
   let r2 = sub pkey nLen nLen in
@@ -504,28 +518,28 @@ let rsapss_verify_lemma a modBits eBits pkey sLen sgnt msgLen msg =
   let emBits = modBits - 1 in
   let emLen = blocks emBits 8 in
 
-  blocks_bits_lemma modBits;
-  assert (blocks k 8 == nLen);
-  assert (8 * blocks k 8 <= max_size_t);
+  blocks_bits_lemma t modBits;
+  assert (blocks k numb == nLen);
   let s = bn_from_bytes_be k sgnt in
-  bn_from_bytes_be_lemma k sgnt;
+  bn_from_bytes_be_lemma #t k sgnt;
 
   let mask = bn_lt_mask s n in
   bn_lt_mask_lemma s n;
 
   let res =
-  if BB.unsafe_bool_of_u64 mask then begin
+  if BB.unsafe_bool_of_limb mask then begin
     let m = bn_mod_exp_precompr2 nLen n s eBits e r2 in
-    Math.Lemmas.pow2_le_compat (64 * nLen) modBits;
-    SM.precomp_r2_mod_n_lemma n;
+    Math.Lemmas.pow2_le_compat (bits * nLen) modBits;
+    SM.bn_precomp_r2_mod_n_lemma n;
     bn_mod_exp_precompr2_lemma nLen n s eBits e r2;
-    em_blocks_lt_max_size_t modBits;
-    assert (8 * blocks emLen 8 <= max_size_t);
+    blocks_bits_lemma t emBits;
+    assert (blocks emLen numb == blocks emBits bits);
 
     bn_lt_pow2_lemma modBits m;
+    assert (bn_lt_pow2 modBits m ==( bn_v m < pow2 (emLen * 8)));
     let res =
     if bn_lt_pow2 modBits m then begin
-      let m1 = sub m 0 (blocks emLen 8) in
+      let m1 = sub m 0 (blocks emLen numb) in
       bn_eval_sub modBits m;
       assert (bn_v m1 == bn_v m);
       let em = bn_to_bytes_be emLen m1 in
@@ -537,10 +551,11 @@ let rsapss_verify_lemma a modBits eBits pkey sLen sgnt msgLen msg =
 
 
 val rsapss_verify:
-    a:Hash.algorithm{S.hash_is_supported a}
+    #t:limb_t
+  -> a:Hash.algorithm{S.hash_is_supported a}
   -> modBits:size_nat
-  -> eBits:size_nat{pkey_len_pre modBits eBits}
-  -> pkey:lbignum (2 * blocks modBits 64 + blocks eBits 64)
+  -> eBits:size_nat{pkey_len_pre t modBits eBits}
+  -> pkey:lbignum t (2 * blocks modBits (bits t) + blocks eBits (bits t))
   -> sLen:size_nat //saltLen
   -> k:size_nat
   -> sgnt:lseq uint8 k
@@ -550,7 +565,7 @@ val rsapss_verify:
   (requires rsapss_pkey_pre modBits eBits pkey)
   (ensures  fun r -> rsapss_verify_post1 a modBits eBits pkey sLen k sgnt msgLen msg r)
 
-let rsapss_verify a modBits eBits pkey sLen k sgnt msgLen msg =
+let rsapss_verify #t a modBits eBits pkey sLen k sgnt msgLen msg =
   let hLen = Hash.hash_length a in
   Math.Lemmas.pow2_lt_compat 61 32;
   Math.Lemmas.pow2_lt_compat 125 32;
@@ -570,30 +585,30 @@ let rsapss_verify a modBits eBits pkey sLen k sgnt msgLen msg =
 
 
 
-val bn_check_num_bits: bits:size_pos -> b:lbignum (blocks bits 64) ->
-  res:uint64{v res == (if bn_v b < pow2 bits then v (ones U64 SEC) else v (zeros U64 SEC))}
+val bn_check_num_bits: #t:limb_t -> bs:size_pos -> b:lbignum t (blocks bs (bits t)) ->
+  res:limb t{v res == (if bn_v b < pow2 bs then v (ones t SEC) else v (zeros t SEC))}
 
-let bn_check_num_bits bits b =
-  let bLen = blocks bits 64 in
-  assert (bits <= 64 * bLen);
-  let m : uint64 = if bits = 64 * bLen then ones U64 SEC else bn_lt_pow2_mask b bits in
-  (if bits = 64 * bLen then begin
+let bn_check_num_bits #t bs b =
+  let bLen = blocks bs (bits t) in
+  assert (bs <= bits t * bLen);
+  let m : limb t = if bs = bits t * bLen then ones t SEC else bn_lt_pow2_mask b bs in
+  (if bs = bits t * bLen then begin
     bn_eval_bound b bLen;
-    Math.Lemmas.pow2_le_compat (64 * bLen) bits end
+    Math.Lemmas.pow2_le_compat (bits t * bLen) bs end
   else
-    bn_lt_pow2_mask_lemma b bits);
-  assert (v m == (if bn_v b < pow2 bits then v (ones U64 SEC) else v (zeros U64 SEC)));
+    bn_lt_pow2_mask_lemma b bs);
+  assert (v m == (if bn_v b < pow2 bs then v (ones t SEC) else v (zeros t SEC)));
   m
 
 
-val rsapss_check_modulus: modBits:size_pos -> n:lbignum (blocks modBits 64) ->
-  res:uint64{v res == (if (bn_v n % 2 = 1 && pow2 (modBits - 1) < bn_v n && bn_v n < pow2 modBits) then v (ones U64 SEC) else v (zeros U64 SEC))}
+val rsapss_check_modulus: #t:limb_t -> modBits:size_pos -> n:lbignum t (blocks modBits (bits t)) ->
+  res:limb t{v res == (if (bn_v n % 2 = 1 && pow2 (modBits - 1) < bn_v n && bn_v n < pow2 modBits) then v (ones t SEC) else v (zeros t SEC))}
 
-let rsapss_check_modulus modBits n =
+let rsapss_check_modulus #t modBits n =
   let bit0 = bn_is_odd n in
   bn_is_odd_lemma n;
   assert (v bit0 == bn_v n % 2);
-  let m0 = u64 0 -. bit0 in
+  let m0 = uint #t 0 -. bit0 in
 
   let m1 = bn_gt_pow2_mask n (modBits - 1) in
   bn_gt_pow2_mask_lemma n (modBits - 1);
@@ -605,10 +620,10 @@ let rsapss_check_modulus modBits n =
   m
 
 
-val rsapss_check_exponent: eBits:size_pos -> e:lbignum (blocks eBits 64) ->
-  res:uint64{v res == (if (0 < bn_v e && bn_v e < pow2 eBits) then v (ones U64 SEC) else v (zeros U64 SEC))}
+val rsapss_check_exponent: #t:limb_t -> eBits:size_pos -> e:lbignum t (blocks eBits (bits t)) ->
+  res:limb t{v res == (if (0 < bn_v e && bn_v e < pow2 eBits) then v (ones t SEC) else v (zeros t SEC))}
 
-let rsapss_check_exponent eBits e =
+let rsapss_check_exponent #t eBits e =
   let m0 = bn_is_zero_mask e in
   bn_is_zero_mask_lemma e;
   let m1 = bn_check_num_bits eBits e in
@@ -619,17 +634,19 @@ let rsapss_check_exponent eBits e =
 
 
 val rsapss_load_pkey_post:
-    modBits:size_nat
-  -> eBits:size_nat{pkey_len_pre modBits eBits}
+    #t:limb_t
+  -> modBits:size_nat
+  -> eBits:size_nat{pkey_len_pre t modBits eBits}
   -> nb:lseq uint8 (blocks modBits 8)
   -> eb:lseq uint8 (blocks eBits 8)
-  -> pkey:lbignum (2 * blocks modBits 64 + blocks eBits 64) -> Type0
+  -> pkey:lbignum t (2 * blocks modBits (bits t) + blocks eBits (bits t)) -> Type0
 
-let rsapss_load_pkey_post modBits eBits nb eb pkey =
+let rsapss_load_pkey_post #t modBits eBits nb eb pkey =
+  let bits = bits t in
   let pkey_s = S.rsapss_load_pkey modBits eBits nb eb in
 
-  let nLen = blocks modBits 64 in
-  let eLen = blocks eBits 64 in
+  let nLen = blocks modBits bits in
+  let eLen = blocks eBits bits in
 
   let n  = sub pkey 0 nLen in
   let e  = sub pkey (nLen + nLen) eLen in
@@ -642,20 +659,22 @@ let rsapss_load_pkey_post modBits eBits nb eb pkey =
 
 
 val rsapss_load_skey_post:
-    modBits:size_nat
+    #t:limb_t
+  -> modBits:size_nat
   -> eBits:size_nat
-  -> dBits:size_nat{skey_len_pre modBits eBits dBits}
+  -> dBits:size_nat{skey_len_pre t modBits eBits dBits}
   -> nb:lseq uint8 (blocks modBits 8)
   -> eb:lseq uint8 (blocks eBits 8)
   -> db:lseq uint8 (blocks dBits 8)
-  -> skey:lbignum (2 * blocks modBits 64 + blocks eBits 64 + blocks dBits 64) -> Type0
+  -> skey:lbignum t (2 * blocks modBits (bits t) + blocks eBits (bits t) + blocks dBits (bits t)) -> Type0
 
-let rsapss_load_skey_post modBits eBits dBits nb eb db skey =
+let rsapss_load_skey_post #t modBits eBits dBits nb eb db skey =
+  let bits = bits t in
   let skey_s = S.rsapss_load_skey modBits eBits dBits nb eb db in
 
-  let nLen = blocks modBits 64 in
-  let eLen = blocks eBits 64 in
-  let dLen = blocks dBits 64 in
+  let nLen = blocks modBits bits in
+  let eLen = blocks eBits bits in
+  let dLen = blocks dBits bits in
 
   let n  = sub skey 0 nLen in
   let e  = sub skey (nLen + nLen) eLen in
@@ -669,46 +688,49 @@ let rsapss_load_skey_post modBits eBits dBits nb eb db skey =
 
 
 val rsapss_load_pkey:
-    modBits:size_nat
-  -> eBits:size_nat{pkey_len_pre modBits eBits}
+    #t:limb_t
+  -> modBits:size_nat
+  -> eBits:size_nat{pkey_len_pre t modBits eBits}
   -> nb:lseq uint8 (blocks modBits 8)
   -> eb:lseq uint8 (blocks eBits 8) ->
-  tuple2 bool (lbignum (2 * blocks modBits 64 + blocks eBits 64))
+  tuple2 bool (lbignum t (2 * blocks modBits (bits t) + blocks eBits (bits t)))
 
-let rsapss_load_pkey modBits eBits nb eb =
+let rsapss_load_pkey #t modBits eBits nb eb =
   let n  = bn_from_bytes_be (blocks modBits 8) nb in
-  let r2 = SM.precomp_r2_mod_n n in
+  let r2 = SM.bn_precomp_r2_mod_n n in
   let e  = bn_from_bytes_be (blocks eBits 8) eb in
   let pkey = (n @| r2) @| e in
 
   let m0 = rsapss_check_modulus modBits n in
   let m1 = rsapss_check_exponent eBits e in
   let m = m0 &. m1 in
-  BB.unsafe_bool_of_u64 m, pkey
+  BB.unsafe_bool_of_limb m, pkey
 
 
 val rsapss_load_pkey_lemma:
-    modBits:size_nat
-  -> eBits:size_nat{pkey_len_pre modBits eBits}
+    #t:limb_t
+  -> modBits:size_nat
+  -> eBits:size_nat{pkey_len_pre t modBits eBits}
   -> nb:lseq uint8 (blocks modBits 8)
   -> eb:lseq uint8 (blocks eBits 8) ->
   Lemma
-  (let b, pkey = rsapss_load_pkey modBits eBits nb eb in
+  (let b, pkey = rsapss_load_pkey #t modBits eBits nb eb in
    let pkey_s = S.rsapss_load_pkey modBits eBits nb eb in
    (if b then rsapss_load_pkey_post modBits eBits nb eb pkey else None? pkey_s))
 
-let rsapss_load_pkey_lemma modBits eBits nb eb =
+let rsapss_load_pkey_lemma #t modBits eBits nb eb =
+  let bits = bits t in
   let nbLen = blocks modBits 8 in
   let ebLen = blocks eBits 8 in
 
-  let nLen = blocks modBits 64 in
-  let eLen = blocks eBits 64 in
+  let nLen = blocks modBits bits in
+  let eLen = blocks eBits bits in
 
-  let n  = bn_from_bytes_be nbLen nb in
-  bn_from_bytes_be_lemma nbLen nb;
-  let r2 = SM.precomp_r2_mod_n n in
-  let e  = bn_from_bytes_be ebLen eb in
-  bn_from_bytes_be_lemma ebLen eb;
+  let n  = bn_from_bytes_be #t nbLen nb in
+  bn_from_bytes_be_lemma #t nbLen nb;
+  let r2 = SM.bn_precomp_r2_mod_n n in
+  let e  = bn_from_bytes_be #t ebLen eb in
+  bn_from_bytes_be_lemma #t ebLen eb;
 
   let pkey = (n @| r2) @| e in
   eq_intro (sub pkey 0 nLen) n;
@@ -723,50 +745,53 @@ let rsapss_load_pkey_lemma modBits eBits nb eb =
 
 
 val rsapss_load_skey:
-    modBits:size_nat
+    #t:limb_t
+  -> modBits:size_nat
   -> eBits:size_nat
-  -> dBits:size_nat{skey_len_pre modBits eBits dBits}
+  -> dBits:size_nat{skey_len_pre t modBits eBits dBits}
   -> nb:lseq uint8 (blocks modBits 8)
   -> eb:lseq uint8 (blocks eBits 8)
   -> db:lseq uint8 (blocks dBits 8) ->
-  tuple2 bool (lbignum (2 * blocks modBits 64 + blocks eBits 64 + blocks dBits 64))
+  tuple2 bool (lbignum t (2 * blocks modBits (bits t) + blocks eBits (bits t) + blocks dBits (bits t)))
 
-let rsapss_load_skey modBits eBits dBits nb eb db =
+let rsapss_load_skey #t modBits eBits dBits nb eb db =
   let b, pkey = rsapss_load_pkey modBits eBits nb eb in
-  let d = bn_from_bytes_be (blocks dBits 8) db in
+  let d = bn_from_bytes_be #t (blocks dBits 8) db in
   let skey = pkey @| d in
 
   let m0 = rsapss_check_exponent dBits d in
-  let b1 = b && BB.unsafe_bool_of_u64 m0 in
+  let b1 = b && BB.unsafe_bool_of_limb m0 in
   b1, skey
 
 
 val rsapss_load_skey_lemma:
-    modBits:size_nat
+    #t:limb_t
+  -> modBits:size_nat
   -> eBits:size_nat
-  -> dBits:size_nat{skey_len_pre modBits eBits dBits}
+  -> dBits:size_nat{skey_len_pre t modBits eBits dBits}
   -> nb:lseq uint8 (blocks modBits 8)
   -> eb:lseq uint8 (blocks eBits 8)
   -> db:lseq uint8 (blocks dBits 8) ->
   Lemma
-  (let b, skey = rsapss_load_skey modBits eBits dBits nb eb db in
+  (let b, skey = rsapss_load_skey #t modBits eBits dBits nb eb db in
    let skey_s = S.rsapss_load_skey modBits eBits dBits nb eb db in
    (if b then rsapss_load_skey_post modBits eBits dBits nb eb db skey else None? skey_s))
 
-let rsapss_load_skey_lemma modBits eBits dBits nb eb db =
+let rsapss_load_skey_lemma #t modBits eBits dBits nb eb db =
+  let bits = bits t in
   let nbLen = blocks modBits 8 in
   let ebLen = blocks eBits 8 in
   let dbLen = blocks dBits 8 in
 
-  let nLen = blocks modBits 64 in
-  let eLen = blocks eBits 64 in
-  let dLen = blocks dBits 64 in
+  let nLen = blocks modBits bits in
+  let eLen = blocks eBits bits in
+  let dLen = blocks dBits bits in
 
-  let b, pkey = rsapss_load_pkey modBits eBits nb eb in
-  rsapss_load_pkey_lemma modBits eBits nb eb;
+  let b, pkey = rsapss_load_pkey #t modBits eBits nb eb in
+  rsapss_load_pkey_lemma #t modBits eBits nb eb;
 
-  let d = bn_from_bytes_be (blocks dBits 8) db in
-  bn_from_bytes_be_lemma (blocks dBits 8) db;
+  let d = bn_from_bytes_be #t (blocks dBits 8) db in
+  bn_from_bytes_be_lemma #t (blocks dBits 8) db;
 
   let skey = pkey @| d in
   eq_intro (sub skey 0 (nLen + nLen + eLen)) pkey;
@@ -774,10 +799,11 @@ let rsapss_load_skey_lemma modBits eBits dBits nb eb db =
 
 
 val rsapss_skey_sign:
-    a:Hash.algorithm{S.hash_is_supported a}
+    #t:limb_t
+  -> a:Hash.algorithm{S.hash_is_supported a}
   -> modBits:size_nat
   -> eBits:size_nat
-  -> dBits:size_nat{skey_len_pre modBits eBits dBits}
+  -> dBits:size_nat{skey_len_pre t modBits eBits dBits}
   -> nb:lseq uint8 (blocks modBits 8)
   -> eb:lseq uint8 (blocks eBits 8)
   -> db:lseq uint8 (blocks dBits 8)
@@ -792,9 +818,9 @@ val rsapss_skey_sign:
    (let sgnt_s = S.rsapss_skey_sign a modBits eBits dBits nb eb db sLen salt msgLen msg in
     if b then Some? sgnt_s /\ sgnt == Some?.v sgnt_s else None? sgnt_s))
 
-let rsapss_skey_sign a modBits eBits dBits nb eb db sLen salt msgLen msg sgnt =
-  let b, skey = rsapss_load_skey modBits eBits dBits nb eb db in
-  rsapss_load_skey_lemma modBits eBits dBits nb eb db;
+let rsapss_skey_sign #t a modBits eBits dBits nb eb db sLen salt msgLen msg sgnt =
+  let b, skey = rsapss_load_skey #t modBits eBits dBits nb eb db in
+  rsapss_load_skey_lemma #t modBits eBits dBits nb eb db;
 
   if b then
     rsapss_sign a modBits eBits dBits skey sLen salt msgLen msg sgnt
@@ -803,9 +829,10 @@ let rsapss_skey_sign a modBits eBits dBits nb eb db sLen salt msgLen msg sgnt =
 
 
 val rsapss_pkey_verify:
-    a:Hash.algorithm{S.hash_is_supported a}
+    #t:limb_t
+  -> a:Hash.algorithm{S.hash_is_supported a}
   -> modBits:size_nat
-  -> eBits:size_nat{pkey_len_pre modBits eBits}
+  -> eBits:size_nat{pkey_len_pre t modBits eBits}
   -> nb:lseq uint8 (blocks modBits 8)
   -> eb:lseq uint8 (blocks eBits 8)
   -> sLen:size_nat //saltLen
@@ -818,9 +845,9 @@ val rsapss_pkey_verify:
   (ensures  fun r ->
     r == S.rsapss_pkey_verify a modBits eBits nb eb sLen k sgnt msgLen msg)
 
-let rsapss_pkey_verify a modBits eBits nb eb sLen k sgnt msgLen msg =
-  let b, pkey = rsapss_load_pkey modBits eBits nb eb in
-  rsapss_load_pkey_lemma modBits eBits nb eb;
+let rsapss_pkey_verify #t a modBits eBits nb eb sLen k sgnt msgLen msg =
+  let b, pkey = rsapss_load_pkey #t modBits eBits nb eb in
+  rsapss_load_pkey_lemma #t modBits eBits nb eb;
 
   if b then
     rsapss_verify a modBits eBits pkey sLen k sgnt msgLen msg
